examples/logic/ltl/concrRepScript.sml
@@ -1,4 +1,4 @@
-open HolKernel Parse bossLib boolLib gfgTheory listTheory optionTheory pred_setTheory rich_listTheory
+open HolKernel Parse bossLib boolLib gfgTheory listTheory optionTheory pred_setTheory rich_listTheory sortingTheory relationTheory
 
 open alterATheory sptreeTheory ltlTheory generalHelpersTheory
 
@@ -514,12 +514,37 @@ val EMPTY_FLWS_LEMM = store_thm
       )
   );
 
+val flws_sorted_def = Define `
+  flws_sorted g =
+    (!x_id fls. x_id ∈ domain g.nodeInfo
+   ∧ (lookup x_id g.followers = SOME fls)
+   ==> (SORTED (λf1 f2. (FST f2).edge_grp <= (FST f1).edge_grp) fls))`;
+
+val FLWS_SORTED_EMPTY = store_thm
+  ("FLWS_SORTED_EMPTY",
+   ``flws_sorted empty``,
+   fs[flws_sorted_def] >> rpt strip_tac >> fs[empty_def,domain_def,foldi_def]
+  );
+
 val first_flw_has_max_counter_def = Define`
   first_flw_has_max_counter g =
      (!x_id fls fl. x_id ∈ domain g.nodeInfo
                ∧ (lookup x_id g.followers = SOME (fl::fls))
                ==> (!y. MEM y fls
                         ==> ((FST y).edge_grp <= (FST fl).edge_grp)))`;
+
+val FLWS_SORTED_IMP_FFHMC = store_thm
+  ("FLWS_SORTED_IMP_FFHMC",
+   ``!g. flws_sorted g ==> first_flw_has_max_counter g``,
+   fs[flws_sorted_def,first_flw_has_max_counter_def] >> rpt strip_tac
+   >> first_x_assum (qspec_then `x_id` mp_tac) >> simp[] >> rpt strip_tac
+   >> qabbrev_tac `P =
+        (λ(f1:β edgeLabelAA # num) (f2:β edgeLabelAA # num).
+          (FST f2).edge_grp ≤ (FST f1).edge_grp)`
+   >> `transitive P` by (qunabbrev_tac `P` >> simp[transitive_def])
+   >> `!y. MEM y fls ==> P fl y` by metis_tac[SORTED_EQ]
+   >> `P fl y` by metis_tac[] >> qunabbrev_tac `P` >> fs[]
+  );
 
 val FIRST_FLW_EMPTY = store_thm
   ("FIRST_FLW_EMPTY",
@@ -547,11 +572,14 @@ val ADDFRML_WFG = store_thm
 
 val ADDFRML_FLW_LEMM = store_thm
   ("ADDFRML_FLW_LEMM",
-  ``!g f. wfg g ∧ first_flw_has_max_counter g
-           ==> first_flw_has_max_counter (addFrmlToGraph g f)``,
-   rpt strip_tac >> fs[first_flw_has_max_counter_def] >> rpt strip_tac
+  ``!g f. wfg g (* ∧ first_flw_has_max_counter g *)
+        ∧ flws_sorted g
+           ==> flws_sorted (addFrmlToGraph g f)(* first_flw_has_max_counter (addFrmlToGraph g f) *)``,
+   (* rpt strip_tac >> fs[first_flw_has_max_counter_def] >> rpt strip_tac *)
+   rpt strip_tac >> fs[flws_sorted_def] >> rpt strip_tac
    >> `wfg (addFrmlToGraph g f)` by metis_tac[ADDFRML_WFG]
-   >> `lookup x_id g.followers = SOME (fl::fls)
+   >> Cases_on `fls` >> fs[SORTED_NIL]
+   >> `lookup x_id g.followers = SOME (h::t)
      ∧ (x_id ∈ domain g.nodeInfo)` by (
        Cases_on `MEM f (MAP ((λl. l.frml) ∘ SND) (toAList g.nodeInfo))`
        >> Cases_on `f` >> fs[addFrmlToGraph_def]
@@ -1008,9 +1036,12 @@ val ADDFRML_FOLDR_LEMM = store_thm
          ∧ (unique_node_formula g
              ==> unique_node_formula
                     (FOLDR (\f g. addFrmlToGraph g f) g fs))
-         ∧ (first_flw_has_max_counter g
-             ==> first_flw_has_max_counter
+         ∧ (flws_sorted g
+             ==> flws_sorted
                     (FOLDR (\f g. addFrmlToGraph g f) g fs))
+         (* ∧ (first_flw_has_max_counter g *)
+         (*     ==> first_flw_has_max_counter *)
+         (*            (FOLDR (\f g. addFrmlToGraph g f) g fs)) *)
          ∧ (wfg g ∧ unique_node_formula g ==>
                 (!x. extractTrans g x =
                        extractTrans (FOLDR (\f g. addFrmlToGraph g f) g fs) x))
@@ -1247,15 +1278,17 @@ val ADD_0EDGE_LEMM = store_thm
 val ADDEDGE_COUNTER_LEMM = store_thm
   ("ADDEDGE_COUNTER_LEMM",
    ``!g e f g2.
-       (addEdgeToGraph f e g = SOME g2) ∧ first_flw_has_max_counter g ∧ wfg g
-          ==> first_flw_has_max_counter g2``,
+       (addEdgeToGraph f e g = SOME g2) ∧ flws_sorted g(* first_flw_has_max_counter g *) ∧ wfg g
+          ==> flws_sorted g2(* first_flw_has_max_counter g2 *)``,
    rpt strip_tac >> Cases_on `e`
-   >> fs[addEdgeToGraph_def,first_flw_has_max_counter_def]
+   >> fs[addEdgeToGraph_def,flws_sorted_def](* fs[addEdgeToGraph_def,first_flw_has_max_counter_def] *)
    >> Cases_on `l1 = []` >> rpt strip_tac >> fs[]
    >- (Cases_on `x` >> fs[]
        >> metis_tac[updateNode_preserves_domain, updateNode_preserves_edges]
       )
-   >- (Cases_on `x` >> fs[]
+   >- ((* Q.HO_MATCH_ABBREV_TAC `SORTED P fls` *)
+       (* >> `transitive P` by (qunabbrev_tac `P` >> simp[transitive_def]) *)
+       Cases_on `x` >> fs[]
        >> qabbrev_tac `LABEL =
            <|edge_grp :=
               (if oldSucPairs = [] then 1n
@@ -1274,7 +1307,8 @@ val ADDEDGE_COUNTER_LEMM = store_thm
                          (CAT_OPTIONS
                           (MAP (λs. findNode (λ(n,l). l.frml = s) g) l))))`
        >> `!ls. ?m. (FOLDR addSingleEdge (SOME g) (TO_LABELS ls) = SOME m)
-                  ∧ (first_flw_has_max_counter m)
+                  (* ∧ (first_flw_has_max_counter m) *)
+                  ∧ (flws_sorted m)
                   ∧ (!fl fls. lookup q m.followers = SOME (fl::fls)
                                ==> (FST fl).edge_grp <= LABEL.edge_grp
                     )
@@ -1283,12 +1317,13 @@ val ADDEDGE_COUNTER_LEMM = store_thm
                   ∧ (g.nodeInfo = m.nodeInfo)
                   ∧ wfg m` by (
             Induct_on `ls`
-            >- (fs[first_flw_has_max_counter_def] >> rpt strip_tac
-                >> `TO_LABELS [] = []` by (
+            >- ((* fs[first_flw_has_max_counter_def] >> rpt strip_tac *)
+                  (* fs[flws_sorted_def] >> rpt strip_tac *)
+                (* >>  *)`TO_LABELS [] = []` by (
                  qunabbrev_tac `TO_LABELS` >> fs[CAT_OPTIONS_def]
                 )
-                >> fs[] >> strip_tac
-                >- metis_tac[]
+                >> fs[] >> strip_tac (* >> qunabbrev_tac `P` *)
+                >- metis_tac[flws_sorted_def]
                 >- (Cases_on `oldSucPairs` >> fs[] >> qunabbrev_tac `LABEL`
                     >> fs[]
                    )
@@ -1331,28 +1366,41 @@ val ADDEDGE_COUNTER_LEMM = store_thm
                      )
                     >> qexists_tac `k` >> fs[]
                     >> qunabbrev_tac `addSingleEdge` >> fs[addEdge_def]
-                    >> fs[gfg_component_equality,
-                          first_flw_has_max_counter_def]
+                    >> fs[gfg_component_equality,flws_sorted_def]
+                          (* first_flw_has_max_counter_def] *)
                     >> rpt strip_tac >> rw[]
                     >> Cases_on `x_id' = q` >> rw[]
-                    >- (`(fl'::fls') = (LABEL,q')::followers_old`
+                    >- ((* `(fl'::fls') = (LABEL,q')::followers_old` *)
+                        (*   by metis_tac[lookup_insert,SOME_11] *)
+                        Q.HO_MATCH_ABBREV_TAC `SORTED P fls'`
+                        >> `transitive P`
+                            by (qunabbrev_tac `P` >> simp[transitive_def])
+                        >> `fls' = (LABEL,q')::followers_old`
                           by metis_tac[lookup_insert,SOME_11]
-                        >> rw[] >> Cases_on `fls'` >> fs[]
-                        >> `(FST y').edge_grp ≤ (FST h').edge_grp`
-                           by metis_tac[]
-                        >> fs[]
-                       )
-                    >- (`lookup x_id' m.followers = SOME (fl'::fls')`
+                        >> rw[] >> fs[] >> rw[]
+                        >> `SORTED
+                             P
+                             followers_old` by metis_tac[]
+                        >> qunabbrev_tac `P` >> Cases_on `followers_old` >> fs[]
+                        >> simp[SORTED_DEF] >> qunabbrev_tac `P` >> fs[]
+                     )
+                       (* (* >> Cases_on `fls'` >> fs[] *) *)
+                       (*  >> `(FST y').edge_grp ≤ (FST h').edge_grp` *)
+                       (*     by metis_tac[] *)
+                       (*  >> fs[] *)
+                    >- ((* `lookup x_id' m.followers = SOME (fl'::fls')` *)
+                        (*       by metis_tac[lookup_insert] *)
+                        `lookup x_id' m.followers = SOME fls'`
                               by metis_tac[lookup_insert]
                         >> `x_id' ∈ domain m.nodeInfo`
                               by metis_tac[domain_lookup,wfg_def]
                         >> metis_tac[]
                        )
-                    >- (`(fl'::fls') = (LABEL,q')::followers_old`
+                    >- (`(fl::fls') = (LABEL,q')::followers_old`
                          by metis_tac[lookup_insert,SOME_11]
                         >> rw[] >> fs[]
                        )
-                    >- (`(fl'::fls') = (LABEL,q')::followers_old`
+                    >- (`(fl::fls') = (LABEL,q')::followers_old`
                          by metis_tac[lookup_insert,SOME_11]
                         >> rw[] >> fs[]
                        )
@@ -1360,11 +1408,11 @@ val ADDEDGE_COUNTER_LEMM = store_thm
                     >- metis_tac[lookup_insert]
                    )
                )
-        )
+       )
        >> first_x_assum (qspec_then `l1` mp_tac)
        >> qunabbrev_tac `TO_LABELS` >> simp[] >> rpt strip_tac
-       >> fs[first_flw_has_max_counter_def] >> metis_tac[]
-      )
+       >> fs[flws_sorted_def] >>  metis_tac[]
+   )
   );
 
 val ADDEDGE_FINAL_LEMM = store_thm
@@ -1422,7 +1470,8 @@ val ADDEDGE_LEMM = store_thm
    ``!g f e aP. wfg g ∧ MEM f (graphStates g)
             ∧ unique_node_formula g
             ∧ (!x. MEM x e.sucs ==> MEM x (graphStates g))
-            ∧ (first_flw_has_max_counter g)
+            ∧ (flws_sorted g)
+            (* ∧ (first_flw_has_max_counter g) *)
         ==> (?g2. (addEdgeToGraph f e g = SOME g2) ∧ wfg g2
           ∧ (set (graphStatesWithId g) = set (graphStatesWithId g2))
           ∧ (unique_node_formula g2)
@@ -1431,7 +1480,8 @@ val ADDEDGE_LEMM = store_thm
                  then ?i. extractTrans g2 h
                         = extractTrans g h ∪ { (i, e.pos,e.neg,set e.sucs) }
                  else extractTrans g2 h = extractTrans g h)
-          ∧ (first_flw_has_max_counter g2))``,
+          ∧ flws_sorted g2
+(* ∧ (first_flw_has_max_counter g2) *))``,
    rpt strip_tac >> Cases_on `e` >> fs[addEdgeToGraph_def]
    >> fs[graphStates_def,MEM_MAP] (* >> simp[findNode_def] *)
    >> `l1 = [] \/ ?h t. l1 = SNOC h t` by metis_tac[SNOC_CASES]
@@ -1931,7 +1981,12 @@ val ADDEDGE_LEMM = store_thm
            >- (disj2_tac >> fs[] >> qexists_tac `l'` >> fs[])
          )
          )
-      >- metis_tac[FIRST_FLW_LEMM,updateNode_preserves_domain]
+      >- (fs[flws_sorted_def] >> rpt strip_tac
+          >> `domain g.nodeInfo = domain x.nodeInfo`
+                by metis_tac[updateNode_preserves_domain]
+          >> metis_tac[]
+         )
+      (* >- metis_tac[FIRST_FLW_LEMM,updateNode_preserves_domain,FLWS_SORTED_IMP_FFHMC] *)
    )
    >- (
     (* Q.HO_MATCH_ABBREV_TAC *)
@@ -1984,6 +2039,7 @@ val ADDEDGE_LEMM = store_thm
             >> `?s_fr. s_fr ∈ s` by fs[MEMBER_NOT_EMPTY]
             >> fs[] >> rw[] >> fs[] >> qunabbrev_tac `LABEL`
             >> fs[theorem "edgeLabelAA_component_equality"] >> rw[]
+            >> `first_flw_has_max_counter g` by metis_tac[FLWS_SORTED_IMP_FFHMC]
             >> fs[first_flw_has_max_counter_def] >> rw[]
             >> `∀y. MEM y t' ⇒ (FST y).edge_grp ≤ (FST h').edge_grp`
                by (
@@ -2015,7 +2071,8 @@ val ADDEDGE_LEMM = store_thm
                              = (extractTrans g a
                                 ∪ { (LABEL.edge_grp,l,l0,h INSERT set fs)})
                        else extractTrans m a = extractTrans g a)
-                   ∧ (first_flw_has_max_counter m)
+                   (* ∧ (first_flw_has_max_counter m) *)
+                   ∧ (flws_sorted m)
                    ∧ (!x id fls q r.
                          findNode (λ(n,l). l.frml = f) m = SOME (q,r)
                        ∧ (lookup q m.followers = SOME fls)
@@ -2052,6 +2109,7 @@ val ADDEDGE_LEMM = store_thm
                           ⇒ lookup o_id k.nodeInfo = lookup o_id g.nodeInfo)`
             by (
             qunabbrev_tac `addSingleEdge` >> fs[addEdge_def]
+            >> `first_flw_has_max_counter g` by metis_tac[FLWS_SORTED_IMP_FFHMC]
             >> simp[first_flw_has_max_counter_def] >> rpt strip_tac
             >> `(q,r) = (nId,frml)` by fs[findNode_def]
             >> Cases_on `followers_old` >> fs[first_flw_has_max_counter_def]
@@ -2068,10 +2126,10 @@ val ADDEDGE_LEMM = store_thm
                >> rw[] >> fs[]
                >> metis_tac[DECIDE``!x y z. x <= y ∧ y <= z ==> x <= z``])
         )
-        >> `first_flw_has_max_counter k` by (
+        >> `flws_sorted k` by (
             qunabbrev_tac `addSingleEdge` >> fs[addEdge_def]
-            >> simp[first_flw_has_max_counter_def] >> rpt strip_tac
-            >> first_x_assum (qspec_then `(LABEL,FST n)::followers_old` mp_tac)
+            >> fs[flws_sorted_def] >> rpt strip_tac
+            >> first_x_assum (qspec_then `fls` mp_tac)
             >> rpt strip_tac
             >> first_x_assum (qspec_then `nId` mp_tac) >> rpt strip_tac
             >> first_x_assum (qspec_then `frml` mp_tac)
@@ -2081,13 +2139,40 @@ val ADDEDGE_LEMM = store_thm
                by (fs[gfg_component_equality]
                    >> metis_tac[lookup_insert,SOME_11])
             >> simp[] >> rpt strip_tac
+            >> Q.HO_MATCH_ABBREV_TAC `SORTED P fls`
+            >> `SORTED P followers_old` by metis_tac[]
             >> Cases_on `x_id = nId` >> fs[gfg_component_equality]
             >> rw[]
-            >> `lookup x_id g.followers = SOME (fl::fls)` by (
-                metis_tac[lookup_insert,SOME_11]
-            )
-            >> fs[first_flw_has_max_counter_def] >> metis_tac[]
+            >- (Cases_on `followers_old` >> fs[] >> simp[SORTED_DEF]
+                >> qunabbrev_tac `P` >> fs[]
+               )
+            >- (`lookup x_id g.followers = SOME fls` by (
+                   metis_tac[lookup_insert,SOME_11]
+                 )
+                >> metis_tac[]
+               )
         )
+        (* >> `first_flw_has_max_counter k` by ( *)
+        (*     qunabbrev_tac `addSingleEdge` >> fs[addEdge_def] *)
+        (*     >> simp[first_flw_has_max_counter_def] >> rpt strip_tac *)
+        (*     >> first_x_assum (qspec_then `(LABEL,FST n)::followers_old` mp_tac) *)
+        (*     >> rpt strip_tac *)
+        (*     >> first_x_assum (qspec_then `nId` mp_tac) >> rpt strip_tac *)
+        (*     >> first_x_assum (qspec_then `frml` mp_tac) *)
+        (*     >> `findNode (λ(n,l). l.frml = (SND y).frml) k = SOME (nId,frml)` *)
+        (*        by metis_tac[findNode_def,SOME_11] *)
+        (*     >> `lookup nId k.followers = SOME ((LABEL,FST n)::followers_old)` *)
+        (*        by (fs[gfg_component_equality] *)
+        (*            >> metis_tac[lookup_insert,SOME_11]) *)
+        (*     >> simp[] >> rpt strip_tac *)
+        (*     >> Cases_on `x_id = nId` >> fs[gfg_component_equality] *)
+        (*     >> rw[] *)
+        (*     >> `lookup x_id g.followers = SOME (fl::fls)` by ( *)
+        (*         metis_tac[lookup_insert,SOME_11] *)
+        (*     ) *)
+        (*     >> `first_flw_has_max_counter g` by metis_tac[FLWS_SORTED_IMP_FFHMC] *)
+        (*     >> fs[first_flw_has_max_counter_def] >> metis_tac[] *)
+        (* ) *)
         >> fs[] >> rpt strip_tac >> fs[]
         >> Cases_on `(SND y).frml = a` >> fs[]
         >- (
@@ -2117,6 +2202,7 @@ val ADDEDGE_LEMM = store_thm
                       >> Cases_on `n` >> rw[] >> fs[]
                       >> rename[`FIND (λ(n,l). l.frml = h) _  = SOME (id,node)`,
                                 `MEM (id,h') (toAList k.nodeInfo)`]
+                      >> `first_flw_has_max_counter g` by metis_tac[FLWS_SORTED_IMP_FFHMC]
                       >- (`(suc = node) ∧ (λ(n,l). l.frml = h) (id,node)`
                             by metis_tac[FIND_LEMM2,MEM_toAList,SOME_11]
                           >> fs[]
@@ -2219,6 +2305,7 @@ val ADDEDGE_LEMM = store_thm
                  >- (qunabbrev_tac `LABEL` >> fs[] >> Cases_on `v`
                      >> fs[] >> Cases_on `h''`
                      >> fs[theorem "edgeLabelAA_component_equality"]
+                     >> `first_flw_has_max_counter g` by metis_tac[FLWS_SORTED_IMP_FFHMC]
                      >> fs[first_flw_has_max_counter_def]
                      >> `∀y. MEM y t'
                           ⇒ (FST y).edge_grp ≤ (FST (q',r')).edge_grp`
@@ -2345,7 +2432,8 @@ val ADDEDGE_LEMM = store_thm
                   extractTrans g (SND y).frml
                                ∪ {(LABEL.edge_grp,l,l0,h INSERT set fs)}
               else extractTrans m a = extractTrans g a)
-              ∧ (first_flw_has_max_counter m)
+              (* ∧ (first_flw_has_max_counter m) *)
+              ∧ (flws_sorted g)
               ∧ (∀fls q r.
                   findNode (λ(n,l). l.frml = (SND y).frml) m = SOME (q,r)
                   ∧ lookup q m.followers = SOME fls
@@ -2362,7 +2450,7 @@ val ADDEDGE_LEMM = store_thm
                      ==> (∀f. MEM f fls ⇒ (FST f).edge_grp ≤ LABEL.edge_grp
                        ∧ (∀o_id. o_id ≠ q
                            ⇒ lookup o_id m1.nodeInfo = lookup o_id g.nodeInfo)))
-                ∧ (first_flw_has_max_counter m1)`
+                ∧ (flws_sorted m1)(* ∧ (first_flw_has_max_counter m1) *)`
              by (
              qunabbrev_tac `addSingleEdge` >> fs[]
              >> Q.HO_MATCH_ABBREV_TAC `
@@ -2391,8 +2479,10 @@ val ADDEDGE_LEMM = store_thm
                 >> fs[gfg_component_equality] >> rw[] >> fs[]
                 >> metis_tac[findNode_def,SOME_11])
              >- (qunabbrev_tac `C`
-                 >> fs[first_flw_has_max_counter_def]
+                 >> fs[flws_sorted_def]
                  >> rpt strip_tac >> fs[]
+                 >> Q.HO_MATCH_ABBREV_TAC `SORTED P fls`
+                 >> `SORTED P followers_old` by metis_tac[]
                  >> first_x_assum (qspec_then `(LABEL,id)::followers_old` mp_tac)
                  >> rpt strip_tac
                  >> first_x_assum (qspec_then `nId` mp_tac) >> rpt strip_tac
@@ -2404,10 +2494,13 @@ val ADDEDGE_LEMM = store_thm
                              >> metis_tac[lookup_insert,SOME_11])
                  >> simp[] >> rpt strip_tac
                  >> Cases_on `x_id = nId` >> fs[gfg_component_equality] >> rw[]
-                 >> `lookup x_id m.followers = SOME (fl::fls)` by (
+                 >- (Cases_on `followers_old` >> qunabbrev_tac `P`
+                     >> simp[SORTED_DEF])
+                 >- (`lookup x_id m.followers = SOME fls` by (
                       metis_tac[lookup_insert,SOME_11]
-                  )
-                 >> fs[first_flw_has_max_counter_def] >> metis_tac[]
+                      )
+                     >> metis_tac[]
+                    )
                 )
          )
          >> qexists_tac `m1` >> fs[] >> rpt strip_tac
@@ -2789,7 +2882,8 @@ val ADDEDGE_FOLDR_LEMM = store_thm
    ``!g1 f. MEM f (graphStates g1)
            ∧ wfg g1
            ∧ unique_node_formula g1
-           ∧ first_flw_has_max_counter g1
+           (* ∧ first_flw_has_max_counter g1 *)
+           ∧ flws_sorted g1
         ==>
        (!ls. ?g2.
         (!e suc. MEM e ls ∧ MEM suc e.sucs
@@ -2797,7 +2891,8 @@ val ADDEDGE_FOLDR_LEMM = store_thm
          ==> ((FOLDR (λe g_opt. monad_bind g_opt (addEdgeToGraph f e))
                   (SOME g1) ls = SOME g2)
             ∧ (wfg g2)
-            ∧ (first_flw_has_max_counter g2)
+            (* ∧ (first_flw_has_max_counter g2) *)
+            ∧ flws_sorted g2
             ∧ (unique_node_formula g2)
             ∧ (set (graphStatesWithId g1)
                 = set (graphStatesWithId g2)))
@@ -2817,7 +2912,8 @@ val ADDEDGE_FOLDR_LEMM = store_thm
      ∧ (set (graphStatesWithId g1)
            = set (graphStatesWithId g2))
      ∧ unique_node_formula g2
-     ∧ first_flw_has_max_counter g2
+     (* ∧ first_flw_has_max_counter g2 *)
+     ∧ flws_sorted g2
      ∧ ∀h.
      if h = f then
          IMAGE SND (extractTrans g2 f) =
@@ -2846,7 +2942,8 @@ val ADDEDGE_FOLDR_LEMM = store_thm
                extractTrans g3 x =
               extractTrans g2 x ∪ {(i,h.pos,h.neg,set h.sucs)}
           else extractTrans g3 x = extractTrans g2 x) ∧
-        first_flw_has_max_counter g3` by metis_tac[ADDEDGE_LEMM]
+        flws_sorted g3
+        (* first_flw_has_max_counter g3 *)` by metis_tac[ADDEDGE_LEMM]
    >> qexists_tac `g3` >> fs[] >> rpt strip_tac >> Cases_on `h' = f` >> fs[]
    >- (rw[] >> first_x_assum (qspec_then `f` mp_tac) >> simp[] >> rpt strip_tac
        >> `IMAGE SND (extractTrans g2 f ∪ {(i,h.pos,h.neg,set h.sucs)})
